theory/JIT_abs.thy
@@ -10,7 +10,7 @@ begin
 record JitProgram =
 page_size     :: usize
 pc_section    :: "usize list"
-text_section  :: "u8 list"
+text_section  :: "x64_bin"
 
 record JitCompiler =
 jit_result :: JitProgram 
@@ -97,42 +97,92 @@ definition per_jit_exit :: "x64_bin option " where
 )"
 
 datatype jit_state =
-  JIT_OK JitCompiler regset SBPFV | (**r normal state *) (*reg_map mem stack_state Config SBPFV*)
-  JIT_Success |
+  JIT_OK JitCompiler| (**r normal state *) (*regset SBPFV  mem Config*)
+  JIT_Success JitProgram|
   JIT_EFlag | (**r find bugs at runtime *)
   JIT_Err (**r bad thing *)
 
-fun per_jit_ins ::" u64 \<Rightarrow> bpf_instruction \<Rightarrow> regset \<Rightarrow> SBPFV \<Rightarrow> x64_bin option"where
-"per_jit_ins pc bins rs sv = (
+fun per_jit_ins ::" bpf_instruction \<Rightarrow> x64_bin option"where
+"per_jit_ins bins = (
   case bins of
   BPF_ALU64 BPF_ADD dst (SOReg src) \<Rightarrow> (per_jit_add_reg64_1 dst src) |
   BPF_EXIT \<Rightarrow> per_jit_exit |
   _ \<Rightarrow> None
 )"
 
+fun per_jit_insns_aux ::"bpf_instruction list \<Rightarrow> x64_bin option list"where
+"per_jit_insns_aux []  = []" |
+"per_jit_insns_aux (x#xs) = (let val = per_jit_ins x in case val of None \<Rightarrow> [None] | _ \<Rightarrow> [val] @ per_jit_insns_aux xs )"
+
+definition per_jit_insns::"bpf_instruction list \<Rightarrow> x64_bin option" where
+"per_jit_insns l = (let l' = per_jit_insns_aux l in 
+                              if last l' = None then None else Some (concat(map Option.the (butlast l'))))"
+
 definition update_pc ::"JitCompiler \<Rightarrow> JitCompiler " where
 "update_pc jcomp = jcomp\<lparr> jit_pc := (jit_pc jcomp) + 1\<rparr>"
 
-definition jit_compile_aux::"u64 \<Rightarrow> bpf_instruction \<Rightarrow> regset \<Rightarrow> SBPFV \<Rightarrow> JitCompiler \<Rightarrow> jit_state" where
-"jit_compile_aux pc bins rs sv jcomp = (let xins = per_jit_ins pc bins rs sv in
-   if bins = BPF_EXIT then JIT_Success else
+definition jit_compile_aux::"u64 \<Rightarrow> bpf_instruction \<Rightarrow> JitCompiler \<Rightarrow> jit_state" where
+"jit_compile_aux pc bins jcomp = (let xins = per_jit_ins bins ; jprog = jit_result jcomp  in
+   if bins = BPF_EXIT then JIT_Success jprog else
    (case xins of None \<Rightarrow> JIT_Err |
                  Some v \<Rightarrow> let jcomp_updated1 = update_pc_section jcomp; jcomp_updated2 = jit_emit jcomp_updated1 v;
                            jcomp_updated = update_pc jcomp_updated2 in 
-    JIT_OK jcomp_updated rs sv))"
-
+    JIT_OK jcomp_updated))"
+                                           
 fun jit_compile :: "nat \<Rightarrow> bpf_bin \<Rightarrow> jit_state \<Rightarrow> jit_state" where
-"jit_compile 0  _ st =  JIT_EFlag " |
+"jit_compile 0 _ st =  JIT_EFlag " |
 "jit_compile (Suc fuel) prog st = (
   case st of 
   JIT_Err \<Rightarrow> JIT_Err |
-  JIT_Success \<Rightarrow> JIT_Success |
+  JIT_Success jprog \<Rightarrow> JIT_Success jprog |
   JIT_EFlag \<Rightarrow> JIT_EFlag |
-  JIT_OK jcomp rs sv \<Rightarrow> ( let pc = jit_pc jcomp in
+  JIT_OK jcomp \<Rightarrow> ( let pc = jit_pc jcomp in
     if unat pc < length prog then
         case bpf_find_instr (unat pc) prog of 
           None \<Rightarrow> JIT_Err |
-          Some ins \<Rightarrow> jit_compile fuel prog (jit_compile_aux pc ins rs sv jcomp)      
+          Some ins \<Rightarrow> jit_compile fuel prog (jit_compile_aux pc ins jcomp)      
     else JIT_Err))"
 
+fun interp3 :: "instruction list \<Rightarrow> outcome \<Rightarrow> outcome" where
+"interp3 [] s = s" |
+"interp3 (ins#l) st = (
+  case st of
+  Stuck \<Rightarrow> Stuck |
+  Next rs m \<Rightarrow> (
+        interp3 l (exec_instr ins 1 rs m)
+))"
+
+datatype bin_state =
+  Bin_OK u64 regset mem | (**r normal state *) (*reg_map mem stack_state Config SBPFV*)
+  Bin_Success|
+  Bin_EFlag | (**r find bugs at runtime *)
+  Bin_Err (**r bad thing *)
+
+definition getInsts::"JitProgram \<Rightarrow> instruction list option" where
+"getInsts jprog = (let insns = text_section jprog in 
+    case x64_decodes 0 insns of None \<Rightarrow> None |
+                                Some v \<Rightarrow> Some (map snd v)) "
+
+fun binary_execute :: "nat \<Rightarrow> JitProgram \<Rightarrow> bin_state \<Rightarrow> bin_state" where
+"binary_execute 0 _ st =  Bin_EFlag " |
+"binary_execute (Suc fuel) jprog st = (
+  case st of 
+  Bin_Err \<Rightarrow> Bin_Err |
+  Bin_Success \<Rightarrow> Bin_Success |
+  Bin_EFlag \<Rightarrow> Bin_EFlag |
+  Bin_OK pc rs m \<Rightarrow> (let v = getInsts jprog in 
+    case v of None \<Rightarrow> Bin_Err |
+              Some insns \<Rightarrow> 
+    if unat pc < length insns then
+      let result = interp3 insns (Next rs m) in 
+        case result of Stuck \<Rightarrow> Bin_EFlag | Next rs' m' \<Rightarrow> Bin_OK (pc+ of_nat(length insns)) rs' m'
+    else Bin_Err))"
+
+
+definition init_jitprog::"JitProgram" where
+"init_jitprog \<equiv> \<lparr> page_size = 4096, pc_section = [], text_section = []\<rparr>"
+
+definition init_jitcomp::"JitCompiler" where
+"init_jitcomp = \<lparr> jit_result = init_jitprog, offset_in_text_section = 0, jit_pc = 0\<rparr>"
+ 
 end
