theory/bpfConsistency.thy
@@ -12,22 +12,11 @@ begin
 
 
 (*JIT_OK JitCompiler reg_map SBPFV *)
-definition is_refined_state :: "bpf_state \<Rightarrow> jit_state \<Rightarrow> bool" where
+(*definition is_refined_state :: "bpf_state \<Rightarrow> jit_state \<Rightarrow> bool" where
 "is_refined_state bst xst = (case bst of BPF_OK pc rs m ss sv fm cur_cu remain_cu \<Rightarrow>
                                 case xst of JIT_OK jcomp res s_v \<Rightarrow> (\<forall> r. Vlong (rs r) = res (IR (bpf_to_x64_reg r))) | _ \<Rightarrow> False |
                                 BPF_Success ret \<Rightarrow> case xst of JIT_Success \<Rightarrow> True | _ \<Rightarrow> False |
                             _ \<Rightarrow> False)"
-
-definition is_refined_state2 :: "bpf_state \<Rightarrow> outcome \<Rightarrow> bool" where
-"is_refined_state2 bst xst = (case bst of BPF_OK pc rs m ss sv fm cur_cu remain_cu \<Rightarrow>
-                                case xst of Next reg mem \<Rightarrow> (\<forall> r. Vlong (rs r) = reg (IR (bpf_to_x64_reg r))) \<and> m = mem | _ \<Rightarrow> False |
-                             BPF_EFlag \<Rightarrow> case xst of Next reg mem \<Rightarrow> False | Stuck \<Rightarrow> True |
-                             BPF_Success ret \<Rightarrow> case xst of Next reg mem \<Rightarrow> reg (IR x64Syntax.RAX) = Vlong ret | 
-                                                            Stuck \<Rightarrow> False |
-                             BPF_Err \<Rightarrow> False)"
-
-(*fun jit_compile :: "nat \<Rightarrow> bpf_bin \<Rightarrow> reg_map \<Rightarrow> jit_state \<Rightarrow> jit_state " where*)
-(*"nat \<Rightarrow> bpf_bin \<Rightarrow> bpf_state \<Rightarrow> bool \<Rightarrow> u64 \<Rightarrow> bpf_state" where*)
 lemma consistency_proof_aux:
   assumes a0:"is_refined_state bst xst" and
     a1:"bst' = bpf_interp fuel prog bst enable_stack_frame_gaps program_vm_addr " and
@@ -35,29 +24,190 @@ lemma consistency_proof_aux:
     a3:"bpf_find_prog 3 0 prog = Some [BPF_ALU64 BPF_ADD BR1 (SOReg BR2), BPF_EXIT]"
   shows "is_refined_state bst' xst'"
   sorry
+*)
+
+(*definition is_refined_state2 :: "bpf_state \<Rightarrow> outcome \<Rightarrow> bool" where
+"is_refined_state2 bst xst = (case bst of BPF_OK pc rs m ss sv fm cur_cu remain_cu \<Rightarrow>
+                                case xst of Next reg mem \<Rightarrow> (\<forall> r. Vlong (rs r) = reg (IR (bpf_to_x64_reg r))) \<and> m = mem | _ \<Rightarrow> False |
+                             BPF_EFlag \<Rightarrow> case xst of Next reg mem \<Rightarrow> False | _ \<Rightarrow> True |
+                             BPF_Success ret \<Rightarrow> case xst of Next reg mem \<Rightarrow> reg (IR x64Syntax.RAX) = Vlong ret | 
+                                                            _ \<Rightarrow> False |
+                             _ \<Rightarrow> False)"
+
+lemma consistency_proof_aux2:
+  assumes a0:"is_refined_state2 bst xst" and
+    a1:"bins = [BPF_ALU64 BPF_ADD BR1 (SOReg BR2), BPF_EXIT] " and
+    a2:"per_jit_insns bins res sv = Some bl" and
+    a3:"list_in_list bl (unat pc) l_bin" and
+    a4:"x64_decodes (unat pc) l_bin = Some v" and
+    a5:"xst' = interp3 xins xst" and
+    a6:"bst' = bpf_interp fuel prog bst enable_stack_frame_gaps program_vm_addr" and
+    a7:"xins = map snd v" and
+    a8:"bpf_find_prog fuel 0 prog = Some bins"
+  shows "is_refined_state2 bst' xst'"
+  sorry
+*)
+
+
+definition is_refined_state2 :: "bpf_state \<Rightarrow> bin_state \<Rightarrow> bool" where
+"is_refined_state2 bst xst = (case bst of BPF_OK pc rs m ss sv fm cur_cu remain_cu \<Rightarrow>
+                                case xst of Bin_OK pc2 reg mem \<Rightarrow> (\<forall> r. Vlong (rs r) = reg (IR (bpf_to_x64_reg r))) | _ \<Rightarrow> False |
+                             BPF_EFlag \<Rightarrow> case xst of Bin_OK pc2 reg mem \<Rightarrow> False | _ \<Rightarrow> True |
+                             BPF_Success ret \<Rightarrow> True |
+                             _ \<Rightarrow> False)"
+  
+
+lemma addq_subgoal_rr_aux1:
+  assumes a0:"bins = BPF_ALU64 BPF_ADD dst (SOReg src)" and
+     a1:"xins = (Paddq_rr (bpf_to_x64_reg dst) (bpf_to_x64_reg src))" and
+     a2:"(BPF_OK pc rs' m ss' is_v1 fm (cur_cu+1) remain_cu) = step fuel bins rs m ss is_v1 fm enable_stack_frame_gaps program_vm_addr cur_cu remain_cu" and
+     a3:"Next reg' m = exec_instr xins sz reg m" and
+     a4:"(\<forall> r. Vlong (rs r) = reg (IR (bpf_to_x64_reg r)))"
+   shows "(\<forall> r. Vlong (rs' r) = reg' (IR (bpf_to_x64_reg r)))"
+proof -
+    have b1:"Vlong (rs dst) = reg (IR (bpf_to_x64_reg dst))" using a4 spec by simp
+    moreover have b2:"Vlong (rs src) = reg (IR (bpf_to_x64_reg src))" using a4 spec by simp
+    hence b3:"Vlong (rs' dst) = reg' (IR (bpf_to_x64_reg dst))" using aluq_subgoal_rr_aux1 a0 a1 a2 a3 b1 b2 by force
+    have b4:"\<forall> r \<noteq> dst. reg'(IR (bpf_to_x64_reg r)) = reg (IR (bpf_to_x64_reg r))" using aluq_subgoal_rr_aux2 a3 a1 by blast
+    have b5:"\<forall> r \<noteq> dst. Vlong (rs' r) = Vlong (rs r)" using a0 a4 aluq_subgoal_rr_aux3 a2 by blast
+    have b6:"\<forall> r \<noteq> dst. Vlong (rs r) = reg (IR (bpf_to_x64_reg r))" using a4 by blast
+    have b7:"(\<forall> r \<noteq> dst. Vlong (rs' r) = reg' (IR (bpf_to_x64_reg r)))" by(simp add:b4 b5 b6) 
+    thus ?thesis using b3 by fastforce
+  qed
+
+
+lemma addq_subgoal_rr_aux2:"bst2 = step 0 (BPF_ALU64 BPF_ADD dst (SOReg src)) rs m ss sv fm enable_stack_frame_gaps program_vm_addr cur_cu remain_cu 
+    \<Longrightarrow> \<exists> rs2. BPF_OK 1 rs2 m ss sv fm (cur_cu+1) remain_cu = bst2"
+  apply(cases "(BPF_ALU64 BPF_ADD dst (SOReg src))",simp_all)
+  apply(unfold eval_alu64_def eval_alu64_aux1_def,simp_all)
+  done
+
+lemma addq_subgoal_rr_aux3:"\<exists> reg2. exec_instr (Paddq_rr (bpf_to_x64_reg dst) (bpf_to_x64_reg src)) 1 reg mem = Next reg2 mem"
+  apply(unfold exec_instr_def)
+  apply(cases "Paddq_rr (bpf_to_x64_reg dst) (bpf_to_x64_reg src)",simp_all)
+  done
+
+(*lemma "bpf_find_prog fuel 0 prog = Some [bins] \<Longrightarrow> bins = BPF_ALU64 BPF_ADD dst (SOReg src) \<Longrightarrow> fuel > 8 \<Longrightarrow> length (bpf_find_prog_aux fuel (0::nat) prog) \<noteq> Suc (0::nat) \<Longrightarrow>
+bpf_find_prog_aux fuel (0::nat) prog = [Some bins, None]"
+  apply(cases bins,simp_all)
+  apply(unfold bpf_find_prog_def Let_def,simp_all)
+  subgoal for x91 apply(split if_splits, simp_all)
+  
+lemma 
+  assumes a0:"bpf_find_prog fuel 0 prog = Some [bins]" and 
+    a1:"bins = BPF_ALU64 BPF_ADD dst (SOReg src)" and 
+    a2:"fuel > 8" 
+  shows" bpf_find_instr 0 prog = Some bins"
+proof-
+  have "bpf_find_prog_aux fuel (0::nat) prog = [Some bins, None]" using a0
+qed
+
+lemma "bpf_find_prog fuel 0 prog = Some [bins] \<Longrightarrow> bins = BPF_ALU64 BPF_ADD dst (SOReg src) \<Longrightarrow> fuel > 8 \<Longrightarrow> bpf_find_instr 0 prog = Some bins"
+  apply(cases bins,simp_all)
+  apply(unfold bpf_find_prog_def Let_def,simp_all)
+  apply(split if_splits, simp_all)
+*)
+
+
+lemma addq_subgoal_rr_aux4:"bpf_find_instr 0 prog = Some bins \<Longrightarrow> prog = [0x95::u8,0x00,0x00,0x00,0x00,0x00,0x00,0x00]
+  \<Longrightarrow> bins = BPF_EXIT"
+  apply(cases bins,simp_all)
+  apply(unfold bpf_find_instr_def rbpf_decoder_def u16_of_u8_list_def u32_of_u8_list_def u4_to_bpf_ireg_def,simp_all)
+  done
+
+lemma addq_subgoal_rr_aux5:"bst = BPF_Success v \<Longrightarrow> bst' = bpf_interp 3 prog bst enable_stack_frame_gaps program_vm_addr \<Longrightarrow> bst = bst'"
+  by (simp add: numeral_3_eq_3)
+
+(*value "bpf_interp 0 [0x95::u8,0x00,0x00,0x00,0x00,0x00,0x00,0x00] (BPF_Success v) enable_stack_frame_gaps program_vm_addr"*)
+
+lemma bpf_interp_list_aux1:
+  assumes a0:"bpf_find_instr 0 prog = Some bins" and
+  a1:"prog = [0x95::u8,0x00,0x00,0x00,0x00,0x00,0x00,0x00]" and
+  a2:"bst' = step 0 bins rs m ss sv fm enable_stack_frame_gaps program_vm_addr cur_cu remain_cu" and
+  a3:"bst' = BPF_Success v" and
+  (*a4:"bst = init_bpf_state init_reg_map init_mem fuel V1"*)
+  a4:"bst = BPF_OK 0 rs m ss sv fm cur_cu remain_cu "
+shows "bst' = bpf_interp 3 prog bst enable_stack_frame_gaps program_vm_addr"
+proof- 
+  have b0:"bins = BPF_EXIT" using addq_subgoal_rr_aux4 a0 a1 by simp
+  have b1:"length prog = 1*INSN_SIZE" using a1 INSN_SIZE_def by auto
+  thus ?thesis using a2 a3 a1 a0 b0 addq_subgoal_rr_aux5 a4 (*init_bpf_state_def init_reg_map_def init_mem_def init_stack_state_def init_func_map_def*)
+    sorry
+  qed
+
+lemma bpf_interp_list_aux2:"bpf_find_prog 3 0 prog = Some bins \<Longrightarrow> 
+  prog = [0x0f::u8,0x12,0x00,0x00,0x00,0x00,0x00,0x00,0x95::u8,0x00,0x00,0x00,0x00,0x00,0x00,0x00] \<Longrightarrow>
+  BPF_OK 1 rs2 m ss sv fm (cur_cu+1) remain_cu = step 0 (bins!0) rs m ss sv fm enable_stack_frame_gaps program_vm_addr cur_cu remain_cu \<Longrightarrow>
+  st2 = step 1 (bins!1) rs2 m ss sv fm enable_stack_frame_gaps program_vm_addr (cur_cu+1) remain_cu \<Longrightarrow>
+  bst' = bpf_interp 3 prog bst enable_stack_frame_gaps program_vm_addr \<Longrightarrow> st2 = bst'"
+  sorry
+
+lemma consistency_proof_aux1:
+  assumes a0:"is_refined_state2 bst xst" and
+    a1:"bins = BPF_ALU64 BPF_ADD dst (SOReg src) " and
+    a2:"bpf_find_instr 0 prog = Some bins" and
+    a3:"bst' = bpf_interp fuel prog bst enable_stack_frame_gaps program_vm_addr" and
+    a4:"JIT_Success jprog = jit_compile fuel' prog (JIT_OK init_jitcomp) " and
+    a5:"xst' = binary_execute fuel' jprog xst" and 
+    a6:"bst = BPF_OK 0 rs m ss sv fm cur_cu remain_cu" and
+    a7:"xst = Bin_OK 0 reg mem" and
+    a8:"mem = m"
+  shows "is_refined_state2 bst' xst'"
+proof - 
+  have "\<exists> bst2. bst2 = step 0 bins rs m ss sv fm enable_stack_frame_gaps program_vm_addr cur_cu remain_cu " by simp
+  obtain bst2 where b1_0:"bst2 = step 0 bins rs m ss sv fm enable_stack_frame_gaps program_vm_addr cur_cu remain_cu " by auto
+  (*have "bpf_find_instr 0 "*)
+  have b1_1:"bins = BPF_ALU64 BPF_ADD dst (SOReg src)" using a1 by simp
+  hence b1_2:"\<exists> rs2. BPF_OK 1 rs2 m ss sv fm (cur_cu+1) remain_cu = bst2" using b1_0 b1_1 addq_subgoal_rr_aux2 by simp
+  obtain rs2 where b1:"BPF_OK 1 rs2 m ss sv fm (cur_cu+1) remain_cu = bst2" using b1_2 by auto
+  (*have "\<exists> bst3. bst3 = step 1 (bins!1) rs2 m ss sv fm enable_stack_frame_gaps program_vm_addr (cur_cu+1) remain_cu" by auto
+  obtain bst3 where b2_0:"bst3 = step 1 (bins!1) rs2 m ss sv fm enable_stack_frame_gaps program_vm_addr (cur_cu+1) remain_cu " by auto
+  have b2_1:"(bins!1) = BPF_EXIT" using a1 by simp
+  have b2:"bst3 = bst'" using a1 a2 a3 b2_0 sorry 
+  have b2_1:"length bins = 1" using a1 by simp*)
+  have b2:"bst2 = bst'"  using a2 a3 b1_0 sorry
+  let ?insns = "Paddq_rr (bpf_to_x64_reg dst) (bpf_to_x64_reg src)" 
+  (*have c0_1:"\<exists> reg mem. xst = Bin_OK 0 reg mem"  sorry
+  obtain reg mem where c0:"xst = Bin_OK 0 reg mem" using c0_1 by auto*)
+  have c1_0:"\<exists> reg2. exec_instr ?insns 1 reg mem = Next reg2 mem" using addq_subgoal_rr_aux3 by simp
+  obtain reg2 where c1:"exec_instr ?insns 1 reg mem  = Next reg2 mem" using c1_0 by auto
+  have c2_0:"Bin_OK 1 reg2 mem = xst'" using c1 a5 sorry
+  have c2_1:"(\<forall> r. Vlong (rs r) = reg (IR (bpf_to_x64_reg r)))" using is_refined_state2_def a0 a6 a7 by simp
+  have c2:"(\<forall> r. Vlong (rs2 r) = reg2 (IR (bpf_to_x64_reg r)))" using addq_subgoal_rr_generic a0 c1 c2_1 b1_1 addq_subgoal_rr_aux1 b1 a8 by (metis b1_0 nth_Cons_0)
+  thus ?thesis using c2_0 b2
+    using b1 is_refined_state2_def by force
+qed
 
 
 lemma consistency_proof_aux2:
   assumes a0:"is_refined_state2 bst xst" and
-    a1:"bst' = bpf_interp fuel prog st enable_stack_frame_gaps program_vm_addr " and
-    a2:"per_jit_ins pc bins rs sv = Some bl" and
-    a3:"list_in_list bl (unat pc) l_bin" and
-    a4:"x64_decode (unat pc) l_bin = Some (length l_bin, xins)" and
-    a5:"xst' = interp3 bbin xst" 
+    a1:"bins = [BPF_ALU64 BPF_ADD dst (SOReg src), BPF_EXIT] " and
+    a2:"bpf_find_prog fuel 0 prog = Some bins" and
+    a3:"bst' = bpf_interp fuel prog bst enable_stack_frame_gaps program_vm_addr" and
+    a4:"JIT_Success jprog = jit_compile fuel' prog (JIT_OK init_jitcomp) " and
+    a5:"xst' = binary_execute fuel' jprog xst" and 
+    a6:"bst = BPF_OK 0 rs m ss sv fm cur_cu remain_cu" and
+    a7:"xst = Bin_OK 0 reg mem" and
+    a8:"mem = m"
   shows "is_refined_state2 bst' xst'"
-  sorry
+proof - 
+  have "\<exists> bst2. bst2 = step 0 (bins!0) rs m ss sv fm enable_stack_frame_gaps program_vm_addr cur_cu remain_cu " by simp
+  obtain bst2 where b1_0:"bst2 = step 0 (bins!0) rs m ss sv fm enable_stack_frame_gaps program_vm_addr cur_cu remain_cu " by auto
+  (*have "bpf_find_instr 0 "*)
+  have b1_1:"(bins!0) = BPF_ALU64 BPF_ADD dst (SOReg src)" using a1 by simp
+  hence b1_2:"\<exists> rs2. BPF_OK 1 rs2 m ss sv fm (cur_cu+1) remain_cu = bst2" using b1_0 b1_1 addq_subgoal_rr_aux2 by simp
+  obtain rs2 where b1:"BPF_OK 1 rs2 m ss sv fm (cur_cu+1) remain_cu = bst2" using b1_2 by auto
+  have "\<exists> bst3. bst3 = step 1 (bins!1) rs2 m ss sv fm enable_stack_frame_gaps program_vm_addr (cur_cu+1) remain_cu" by auto
+  obtain bst3 where b2_0:"bst3 = step 1 (bins!1) rs2 m ss sv fm enable_stack_frame_gaps program_vm_addr (cur_cu+1) remain_cu " by auto
+  have b2_1:"(bins!1) = BPF_EXIT" using a1 by simp
+  have b2:"bst3 = bst'" using a1 a2 a3 b2_0 sorry 
+  let ?insns = "[Paddq_rr (bpf_to_x64_reg dst) (bpf_to_x64_reg src),Pret]" 
+  (*have c0_1:"\<exists> reg mem. xst = Bin_OK 0 reg mem"  sorry
+  obtain reg mem where c0:"xst = Bin_OK 0 reg mem" using c0_1 by auto*)
+  have c1_0:"\<exists> reg2. exec_instr (?insns!0) 1 reg mem = Next reg2 mem" using addq_subgoal_rr_aux3 by simp
+  obtain reg2 where c1:"exec_instr (?insns!0) 1 reg mem  = Next reg2 mem" using c1_0 by auto
+  have c2_1:"(\<forall> r. Vlong (rs r) = reg (IR (bpf_to_x64_reg r)))" using is_refined_state2_def a0 a6 a7 by simp
+  have c2:"(\<forall> r. Vlong (rs2 r) = reg2 (IR (bpf_to_x64_reg r)))" using addq_subgoal_rr_generic a0 c1 c2_1 b1_1 addq_subgoal_rr_aux1 b1 a8 by (metis b1_0 nth_Cons_0)
+  thus ?thesis sorry
+qed
 
-
-(*lemma sarq_subgoal_rr_generic:
-  assumes a0:"bins = BPF_ALU64 BPF_ARSH dst (SOReg src)" and
-       a1:"per_jit_shift_reg64 7 dst src = Some bl" and
-       a2:"list_in_list bl (unat pc) l_bin" and
-       a3:"x64_decodes (unat pc) l_bin = Some v" and
-       a4:"(BPF_OK pc rs' m' ss' is_v1 fm (cur_cu+1) remain_cu) = step fuel bins rs m ss is_v1 fm enable_stack_frame_gaps program_vm_addr cur_cu remain_cu" and
-       a5:"Next reg' m' = interp3 xins (Next reg m) " and
-       a6:"(\<forall> r. Vlong (rs r) = reg (IR (bpf_to_x64_reg r)))" and
-       a7:"(bpf_to_x64_reg dst) \<noteq> x64Syntax.RCX" and
-       a8:"xins = map snd v" and
-       a9:"Vlong n1 = reg (IR SP)"
-  shows "(\<forall> r. Vlong (rs' r) = reg' (IR (bpf_to_x64_reg r)))"
-*)
